rocq/ZF/Meta/Shift.v
@@ -31,6 +31,7 @@ Fixpoint fromT (i j:nat) (t:Term) : Term :=
   | Lam p            => Lam   (fromT (S i) j p)
   | App A x          => App   (fromT i j A) (fromT i j x)
   | Def A p q        => Def   (fromT i j A) (fromP i j p) (fromP i j q)
+  | FromC A p        => FromC (fromT i j A) (fromP i j p)
   end
 with fromP (i j:nat) (p:Proof) : Proof :=
   match p with
@@ -79,6 +80,7 @@ Proof.
   - intros p IH i. simpl. rewrite IH. reflexivity.
   - intros A x IH1 IH2 i. simpl. rewrite IH1, IH2. reflexivity.
   - intros A p q IH1 IH2 IH3 i. simpl. rewrite IH1, IH2, IH3. reflexivity.
+  - intros A p IH1 IH2 i. simpl. rewrite IH1, IH2. reflexivity.
   - intros i. reflexivity.
   - intros t ts IH1 IH2 i. simpl. rewrite IH1, IH2. reflexivity.
   - intros t IH i. simpl. rewrite IH. reflexivity.
@@ -210,6 +212,8 @@ Proof.
     rewrite IH1, IH2; try assumption. reflexivity.
   - intros A p q IH1 IH2 IH3 i j k l H1. simpl.
     rewrite IH1, IH2, IH3; try assumption. reflexivity.
+  - intros A p IH1 IH2 i j k l H1. simpl.
+    rewrite IH1, IH2; try assumption. reflexivity.
   - intros i j k l H1. reflexivity.
   - intros t ts IH1 IH2 i j k l H1. simpl.
     rewrite IH1, IH2; try assumption. reflexivity.
@@ -305,6 +309,7 @@ Proof.
   - intros A x IH1 IH2 i j k l. simpl. rewrite IH1, IH2. reflexivity.
   - intros A p q IH1 IH2 IH3 i j k l. simpl.
     rewrite IH1, IH2, IH3. reflexivity.
+  - intros A p IH1 IH2 i j k l. simpl. rewrite IH1, IH2. reflexivity.
   - intros i j k l. reflexivity.
   - intros t ts IH1 IH2 i j k l. simpl. rewrite IH1, IH2. reflexivity.
   - intros t IH i j k l. simpl. rewrite IH. reflexivity.
